I will use the per partes becuase 
I don't see how the sub-method will 
help me here.

\begin{center}
    \textit{Per partes method}
    $$ \int uv' = uv - \int vu' $$
\end{center}

The \textit{per partes} method is derived 
from the product rule in derivation ($(uv)' = u'v + uv'$).

\[
\begin{aligned}
    \text{Výběr funkce $f$:} & \quad f(x) = (2x + 3) \rightarrow f'(x) = 2 \\
    \text{Výběr funkce $g$:} & \quad g'(x) = e^x \rightarrow g(x) = e^x  \\
\end{aligned}
\]

\begin{align}
    \int &(2x + 3)e^x \diff{x} =\\
    &= (2x+3)e^x - 2\int e^x \diff{x} =\\
    &= (2x+3)e^x - 2e^x = \\
    &= e^x(2x + 1) + C 
\end{align}
