\qs{}{
    $$ \lim_{\ntoinf} \frac{(n + 1)! - 2(n!)}{3(n+1)! + 1} $$
}

\begin{align}
    \lim_{\ntoinf} & \frac{(n + 1)!(1 - \frac{2}{n + 1})}{(n + 1)!(3 + \frac{1}{(n + 1)!})} \\
    \lim_{\ntoinf} & \frac{(1 - \frac{2}{n + 1})}{(3 + \frac{1}{(n + 1)!})} \\
    \lim_{\ntoinf} & \frac{1 + 0}{3 + 0} = \frac{1}{3}
\end{align}

\defi{Vytýkání faktoriálu}{
    $$ a(n!) = \frac{a}{n + 1}(n + 1)! $$
    $$ a(n!) = \frac{a}{(n + 2)(n + 1)}(n + 2)! $$
    $$ a(n!) = \frac{a}{(n + 3)(n + 2)(n + 1)}(n + 3)! $$
}

\pagebreak
